src/ssa/ssa_dynamic.v
@@ -434,37 +434,37 @@ Inductive dsInsn : State -> State -> trace -> Prop :=
                       ::EC) gl fs Mem)
     trace_nil
 
-| dsCall : forall S TD Ps F B lc gl fs rid noret tailc fid fv lp cs tmn
-                            l' ps' cs' tmn' EC rt la va lb Mem als ft,
+| dsCall : forall S TD Ps F B lc gl fs rid noret ca fid fv lp cs tmn
+                            l' ps' cs' tmn' EC rt la va lb Mem als ft fa,
   (* only look up the current module for the time being, 
      do not support linkage. *)
   lookupFdefViaGV TD Mem Ps gl lc fs fv = 
-    Some (fdef_intro (fheader_intro rt fid la va) lb) ->
-  getEntryBlock (fdef_intro (fheader_intro rt fid la va) lb) = 
+    Some (fdef_intro (fheader_intro fa rt fid la va) lb) ->
+  getEntryBlock (fdef_intro (fheader_intro fa rt fid la va) lb) = 
     Some (block_intro l' ps' cs' tmn') ->
   dsInsn 
-    (mkState S TD Ps ((mkEC F B ((insn_call rid noret tailc ft fv lp)::cs) tmn 
+    (mkState S TD Ps ((mkEC F B ((insn_call rid noret ca ft fv lp)::cs) tmn 
                        lc als)::EC) gl fs Mem)
-    (mkState S TD Ps ((mkEC (fdef_intro (fheader_intro rt fid la va) lb) 
+    (mkState S TD Ps ((mkEC (fdef_intro (fheader_intro fa rt fid la va) lb) 
                        (block_intro l' ps' cs' tmn') cs' tmn' 
                        (initLocals la (params2GVs TD Mem lp lc gl)) 
                        nil)::
-                      (mkEC F B ((insn_call rid noret tailc ft fv lp)::cs) tmn 
+                      (mkEC F B ((insn_call rid noret ca ft fv lp)::cs) tmn 
                        lc als)::EC) gl fs Mem)
     trace_nil 
 
-| dsExCall : forall S TD Ps F B lc gl fs rid noret tailc fid fv lp cs tmn EC 
-                    rt la Mem als oresult Mem' lc' va ft,
+| dsExCall : forall S TD Ps F B lc gl fs rid noret ca fid fv lp cs tmn EC 
+                    rt la Mem als oresult Mem' lc' va ft fa,
   (* only look up the current module for the time being, 
      do not support linkage. 
      FIXME: should add excall to trace
   *)
   lookupExFdecViaGV TD Mem Ps gl lc fs fv = 
-    Some (fdec_intro (fheader_intro rt fid la va)) ->
+    Some (fdec_intro (fheader_intro fa rt fid la va)) ->
   callExternalFunction Mem fid (params2GVs TD Mem lp lc gl) = (oresult, Mem') ->
   exCallUpdateLocals noret rid oresult lc = Some lc' ->
   dsInsn 
-    (mkState S TD Ps ((mkEC F B ((insn_call rid noret tailc ft fv lp)::cs) tmn 
+    (mkState S TD Ps ((mkEC F B ((insn_call rid noret ca ft fv lp)::cs) tmn 
                        lc als)::EC) gl fs Mem)
     (mkState S TD Ps ((mkEC F B cs tmn lc' als)::EC) gl fs Mem')
     trace_nil 
@@ -501,13 +501,13 @@ match Ps with
   | Some gv => genGlobalAndInitMem TD Ps' (updateAddAL _ gl id0 gv) fs Mem
   | None => None
   end
-| (product_fdef (fdef_intro (fheader_intro _ id0 _ _) _))::Ps' =>
+| (product_fdef (fdef_intro (fheader_intro _ _ id0 _ _) _))::Ps' =>
   match initFunTable Mem id0 with
   | Some gv => genGlobalAndInitMem TD Ps' (updateAddAL _ gl id0 gv) 
       (updateAddAL _ fs id0 gv) Mem
   | None => None
   end
-| (product_fdec (fdec_intro (fheader_intro _ id0 _ _)))::Ps' =>
+| (product_fdec (fdec_intro (fheader_intro _ _ id0 _ _)))::Ps' =>
   match initFunTable Mem id0 with
   | Some gv => genGlobalAndInitMem TD Ps' (updateAddAL _ gl id0 gv) 
       (updateAddAL _ fs id0 gv) Mem
@@ -530,7 +530,7 @@ match (lookupFdefViaIDFromSystem S main) with
       | None => None
       | Some (block_intro l ps cs tmn) => 
           match CurFunction with 
-          | fdef_intro (fheader_intro rt _ la _) _ =>
+          | fdef_intro (fheader_intro _ rt _ la _) _ =>
             let Values := initLocals la Args in
               Some
               (mkState
@@ -852,34 +852,34 @@ Inductive nsInsn : State*trace -> States -> Prop :=
                           else updateAddAL _ lc id gv1) als)::EC) 
                          gl fs Mem, tr)::nil)
 
-| nsCall : forall S TD Ps F B lc gl fs rid noret tailc fv fid lp cs tmn
-                            l' ps' cs' tmn' EC rt id la va lb tr Mem als ft,
+| nsCall : forall S TD Ps F B lc gl fs rid noret fv fid lp cs tmn
+                fa ca l' ps' cs' tmn' EC rt id la va lb tr Mem als ft,
   lookupFdefViaGV TD Mem Ps gl lc fs fv = 
-    Some (fdef_intro (fheader_intro rt fid la va) lb) ->
-  getEntryBlock (fdef_intro (fheader_intro rt fid la va) lb) = 
+    Some (fdef_intro (fheader_intro fa rt fid la va) lb) ->
+  getEntryBlock (fdef_intro (fheader_intro fa rt fid la va) lb) = 
     Some (block_intro l' ps' cs' tmn') ->
   nsInsn 
-    (mkState S TD Ps ((mkEC F B ((insn_call rid noret tailc ft fv lp)::cs) tmn 
+    (mkState S TD Ps ((mkEC F B ((insn_call rid noret ca ft fv lp)::cs) tmn 
                       lc als)::EC) gl fs Mem, tr)
-    ((mkState S TD Ps ((mkEC (fdef_intro (fheader_intro rt id la va) lb) 
+    ((mkState S TD Ps ((mkEC (fdef_intro (fheader_intro fa rt id la va) lb) 
                        (block_intro l' ps' cs' tmn') cs' tmn' 
                          (initLocals la (params2GVs TD Mem lp lc gl)) 
                          nil)::
-                       (mkEC F B ((insn_call rid noret tailc ft fv lp)::cs) tmn 
+                       (mkEC F B ((insn_call rid noret ca ft fv lp)::cs) tmn 
                        lc als)::EC) gl fs Mem, tr)::nil)
 
-| nsExCall : forall S TD Ps F B lc gl fs rid noret tailc fv fid lp cs tmn EC
-                    rt la va Mem als tr oresult Mem' lc' ft,
+| nsExCall : forall S TD Ps F B lc gl fs rid noret ca fv fid lp cs tmn EC
+                    rt la va Mem als tr oresult Mem' lc' ft fa,
   (* only look up the current module for the time being, 
      do not support linkage. 
      FIXME: should add excall to trace
   *)
   lookupExFdecViaGV TD Mem Ps gl lc fs fv = 
-    Some (fdec_intro (fheader_intro rt fid la va)) ->
+    Some (fdec_intro (fheader_intro fa rt fid la va)) ->
   callExternalFunction Mem fid (params2GVs TD Mem lp lc gl) = (oresult, Mem') ->
   exCallUpdateLocals noret rid oresult lc = Some lc' ->
   nsInsn 
-    (mkState S TD Ps ((mkEC F B ((insn_call rid noret tailc ft fv lp)::cs) tmn 
+    (mkState S TD Ps ((mkEC F B ((insn_call rid noret ca ft fv lp)::cs) tmn 
                       lc als)::EC) gl fs Mem, tr)
     ((mkState S TD Ps ((mkEC F B cs tmn lc' als)::EC) gl fs Mem', tr)::nil)
 .
@@ -900,7 +900,7 @@ match (lookupFdefViaIDFromSystem S main) with
       | None => None
       | Some (block_intro l ps cs tmn) => 
           match CurFunction with 
-          | fdef_intro (fheader_intro rt _ la _) _ =>
+          | fdef_intro (fheader_intro _ rt _ la _) _ =>
             let Values := initLocals la Args in
             Some
               ((mkState
@@ -1213,30 +1213,30 @@ Inductive dbInsn : State -> State -> trace -> Prop :=
                        gl fs Mem)
     trace_nil
 
-| dbCall : forall S TD Ps F B lc gl fs rid noret tailc rt fv lp cs tmn
+| dbCall : forall S TD Ps F B lc gl fs rid noret ca rt fv lp cs tmn
                        EC Rid oResult tr B' lc' Mem Mem' als' als Mem'' lc'' ft,
-  dbFdef fv rt lp S TD Ps ((mkEC F B ((insn_call rid noret tailc ft fv lp)::cs)
+  dbFdef fv rt lp S TD Ps ((mkEC F B ((insn_call rid noret ca ft fv lp)::cs)
     tmn lc als)::EC) lc gl fs Mem lc' als' Mem' B' Rid oResult tr ->
   free_allocas TD Mem' als' = Some Mem'' ->
   callUpdateLocals TD Mem'' noret rid oResult lc lc' gl = Some lc'' ->
   dbInsn 
-    (mkState S TD Ps ((mkEC F B ((insn_call rid noret tailc ft fv lp)::cs) tmn 
+    (mkState S TD Ps ((mkEC F B ((insn_call rid noret ca ft fv lp)::cs) tmn 
                        lc als)::EC) gl fs Mem) 
     (mkState S TD Ps ((mkEC F B cs tmn lc'' als)::EC) gl fs Mem'') 
     tr
 
-| dbExCall : forall S TD Ps F B lc gl fs rid noret tailc fv fid lp cs tmn EC
-                    rt la va Mem als oresult Mem' lc' ft,
+| dbExCall : forall S TD Ps F B lc gl fs rid noret fv fid lp cs tmn EC
+                    rt la va Mem als oresult Mem' lc' ft fa ca,
   (* only look up the current module for the time being, 
      do not support linkage. 
      FIXME: should add excall to trace
   *)
   lookupExFdecViaGV TD Mem Ps gl lc fs fv = 
-    Some (fdec_intro (fheader_intro rt fid la va)) ->
+    Some (fdec_intro (fheader_intro fa rt fid la va)) ->
   callExternalFunction Mem fid (params2GVs TD Mem lp lc gl) = (oresult, Mem') ->
   exCallUpdateLocals noret rid oresult lc = Some lc' ->
   dbInsn 
-    (mkState S TD Ps ((mkEC F B ((insn_call rid noret tailc ft fv lp)::cs) tmn 
+    (mkState S TD Ps ((mkEC F B ((insn_call rid noret ca ft fv lp)::cs) tmn 
                        lc als)::EC) gl fs Mem)
     (mkState S TD Ps ((mkEC F B cs tmn lc' als)::EC) gl fs Mem')
     trace_nil
@@ -1251,18 +1251,18 @@ with dbop : State -> State -> trace -> Prop :=
 with dbFdef : value -> typ -> params -> system -> TargetData -> products -> 
             list ExecutionContext -> GVMap -> GVMap -> GVMap -> mem -> GVMap ->
             list mblock -> mem -> block -> id -> option value -> trace -> Prop :=
-| dbFdef_func : forall S TD Ps gl fs fv fid lp lc rid
+| dbFdef_func : forall S TD Ps gl fs fv fid lp lc rid fa
       l' ps' cs' tmn' rt la lb l'' ps'' cs'' Result lc' tr ECs Mem Mem' als' va,
   lookupFdefViaGV TD Mem Ps gl lc fs fv = 
-    Some (fdef_intro (fheader_intro rt fid la va) lb) ->
-  getEntryBlock (fdef_intro (fheader_intro rt fid la va) lb) = 
+    Some (fdef_intro (fheader_intro fa rt fid la va) lb) ->
+  getEntryBlock (fdef_intro (fheader_intro fa rt fid la va) lb) = 
     Some (block_intro l' ps' cs' tmn') ->
   dbop 
-    (mkState S TD Ps ((mkEC (fdef_intro (fheader_intro rt fid la va) lb) 
+    (mkState S TD Ps ((mkEC (fdef_intro (fheader_intro fa rt fid la va) lb) 
                              (block_intro l' ps' cs' tmn') cs' tmn' 
                              (initLocals la (params2GVs TD Mem lp lc gl))
                             nil)::ECs) gl fs Mem)
-    (mkState S TD Ps ((mkEC (fdef_intro (fheader_intro rt fid la va) lb) 
+    (mkState S TD Ps ((mkEC (fdef_intro (fheader_intro fa rt fid la va) lb) 
                              (block_intro l'' ps'' cs'' 
                              (insn_return rid rt Result)) nil 
                              (insn_return rid rt Result) lc'
@@ -1271,18 +1271,18 @@ with dbFdef : value -> typ -> params -> system -> TargetData -> products ->
   dbFdef fv rt lp S TD Ps ECs lc gl fs Mem lc' als' Mem' 
     (block_intro l'' ps'' cs'' (insn_return rid rt Result)) rid (Some Result) tr
 
-| dbFdef_proc : forall S TD Ps gl fs fv fid lp lc rid
+| dbFdef_proc : forall S TD Ps gl fs fv fid lp lc rid fa 
            l' ps' cs' tmn' rt la lb l'' ps'' cs'' lc' tr ECs Mem Mem' als' va,
   lookupFdefViaGV TD Mem Ps gl lc fs fv = 
-    Some (fdef_intro (fheader_intro rt fid la va) lb) ->
-  getEntryBlock (fdef_intro (fheader_intro rt fid la va) lb) = 
+    Some (fdef_intro (fheader_intro fa rt fid la va) lb) ->
+  getEntryBlock (fdef_intro (fheader_intro fa rt fid la va) lb) = 
     Some (block_intro l' ps' cs' tmn') ->
   dbop 
-    (mkState S TD Ps ((mkEC (fdef_intro (fheader_intro rt fid la va) lb) 
+    (mkState S TD Ps ((mkEC (fdef_intro (fheader_intro fa rt fid la va) lb) 
                              (block_intro l' ps' cs' tmn') cs' tmn' 
                              (initLocals la (params2GVs TD Mem lp lc gl))
                             nil)::ECs) gl fs Mem)
-    (mkState S TD Ps ((mkEC (fdef_intro (fheader_intro rt fid la va) lb) 
+    (mkState S TD Ps ((mkEC (fdef_intro (fheader_intro fa rt fid la va) lb) 
                              (block_intro l'' ps'' cs'' (insn_return_void rid)) 
                              nil (insn_return_void rid) lc'
                             als')::ECs) gl fs Mem')
@@ -1292,12 +1292,12 @@ with dbFdef : value -> typ -> params -> system -> TargetData -> products ->
 .
 
 CoInductive dbInsnInf : State -> Trace -> Prop :=
-| dbCallInsnInf : forall S TD Ps F B lc gl fs rid noret tailc rt fv lp cs tmn
+| dbCallInsnInf : forall S TD Ps F B lc gl fs rid noret ca rt fv lp cs tmn
                        EC tr Mem als ft,
-  dbFdefInf fv rt lp S TD Ps ((mkEC F B ((insn_call rid noret tailc ft fv lp)
+  dbFdefInf fv rt lp S TD Ps ((mkEC F B ((insn_call rid noret ca ft fv lp)
     ::cs) tmn lc als)::EC) lc gl fs Mem tr ->
   dbInsnInf 
-    (mkState S TD Ps ((mkEC F B ((insn_call rid noret tailc ft fv lp)::cs) tmn 
+    (mkState S TD Ps ((mkEC F B ((insn_call rid noret ca ft fv lp)::cs) tmn 
       lc als)::EC) gl fs Mem) tr
 
 with dbopInf : State -> Trace -> Prop :=
@@ -1311,14 +1311,14 @@ with dbopInf : State -> Trace -> Prop :=
 
 with dbFdefInf : value -> typ -> params -> system -> TargetData -> products -> 
   list ExecutionContext -> GVMap -> GVMap  -> GVMap -> mem -> Trace -> Prop :=
-| dbFdefInf_intro : forall S TD Ps lc gl fs fv fid lp
+| dbFdefInf_intro : forall S TD Ps lc gl fs fv fid lp fa
                            l' ps' cs' tmn' rt la va lb tr ECs Mem,
   lookupFdefViaGV TD Mem Ps gl lc fs fv = 
-    Some (fdef_intro (fheader_intro rt fid la va) lb) ->
-  getEntryBlock (fdef_intro (fheader_intro rt fid la va) lb) = 
+    Some (fdef_intro (fheader_intro fa rt fid la va) lb) ->
+  getEntryBlock (fdef_intro (fheader_intro fa rt fid la va) lb) = 
     Some (block_intro l' ps' cs' tmn') ->
   dbopInf 
-    (mkState S TD Ps ((mkEC (fdef_intro (fheader_intro rt fid la va) lb) 
+    (mkState S TD Ps ((mkEC (fdef_intro (fheader_intro fa rt fid la va) lb) 
                         (block_intro l' ps' cs' tmn') cs' tmn'
                         (initLocals la (params2GVs TD Mem lp lc gl)) 
                         nil)::ECs) gl fs Mem)
@@ -1358,24 +1358,24 @@ Inductive db_goeswrong : system -> id -> list GenericValue -> State -> Prop :=
 (***************************************************************)
 (* non-deterministic big-step *)
 
-Fixpoint returnStatesFromOp S TD Ps ECs gl fs rt fid la va lb 
+Fixpoint returnStatesFromOp S TD Ps ECs gl fs fa rt fid la va lb 
   (lc_als_Mem_block_ore_trs : 
   list (GVMap*list mblock*mem*block*id*option value*trace)) : States :=
 match lc_als_Mem_block_ore_trs with
 | nil => nil
 | (lc', als', Mem', B'', rid, Some re, tr')::lc_als_Mem_block_ore_trs' => 
-    (mkState S TD Ps ((mkEC (fdef_intro (fheader_intro rt fid la va) lb) 
+    (mkState S TD Ps ((mkEC (fdef_intro (fheader_intro fa rt fid la va) lb) 
                              B'' nil (insn_return rid rt re) lc'
                             als')::ECs) gl fs Mem',
                        tr')::
-    (returnStatesFromOp S TD Ps ECs gl fs rt fid la va lb 
+    (returnStatesFromOp S TD Ps ECs gl fs fa rt fid la va lb 
        lc_als_Mem_block_ore_trs')
 | (lc', als', Mem', B'', rid, None, tr')::lc_als_Mem_block_ore_trs' => 
-    (mkState S TD Ps ((mkEC (fdef_intro (fheader_intro rt fid la va) lb) 
+    (mkState S TD Ps ((mkEC (fdef_intro (fheader_intro fa rt fid la va) lb) 
                              B'' nil (insn_return_void rid) lc'
                             als')::ECs) gl fs Mem',
                        tr')::
-    (returnStatesFromOp S TD Ps ECs gl fs rt fid la va lb 
+    (returnStatesFromOp S TD Ps ECs gl fs fa rt fid la va lb 
       lc_als_Mem_block_ore_trs')
 end.
 
@@ -1607,29 +1607,29 @@ Inductive nbInsn : State*trace -> States -> Prop :=
                           else updateAddAL _ lc id gv1) als)::EC) gl fs Mem, 
                        tr)::nil)
 
-| nbCall : forall S TD Ps F B lc gl fs rid noret tailc rt fv lp cs tmn
+| nbCall : forall S TD Ps F B lc gl fs rid noret ca rt fv lp cs tmn
                          EC tr lc_als_Mem_block_rid_ore_trs Mem als states ft, 
-  nbFdef fv rt lp S TD Ps ((mkEC F B ((insn_call rid noret tailc ft fv lp)::cs) 
+  nbFdef fv rt lp S TD Ps ((mkEC F B ((insn_call rid noret ca ft fv lp)::cs) 
      tmn lc als)::EC) lc gl fs Mem tr lc_als_Mem_block_rid_ore_trs ->
   updateStatesFromReturns S TD Ps F B cs tmn lc gl fs rid als EC noret 
     lc_als_Mem_block_rid_ore_trs = Some states ->
   nbInsn 
-    (mkState S TD Ps ((mkEC F B ((insn_call rid noret tailc ft fv lp)::cs) tmn 
+    (mkState S TD Ps ((mkEC F B ((insn_call rid noret ca ft fv lp)::cs) tmn 
                        lc als)::EC) gl fs Mem, tr) states    
 
-| nbExCall : forall S TD Ps F B lc gl fs rid noret tailc fv fid lp cs tmn EC
-                     rt la va Mem als tr oresult Mem' lc' ft,
+| nbExCall : forall S TD Ps F B lc gl fs rid noret ca fv fid lp cs tmn EC
+                     rt la va Mem als tr oresult Mem' lc' ft fa,
   (* only look up the current module for the time being, 
      do not support linkage. 
      FIXME: should add excall to trace
   *)
   lookupExFdecViaGV TD Mem Ps gl lc fs fv = 
-    Some (fdec_intro (fheader_intro rt fid la va)) ->
+    Some (fdec_intro (fheader_intro fa rt fid la va)) ->
   callExternalFunction Mem fid (params2GVs TD Mem lp lc gl) = (oresult, Mem') ->
   exCallUpdateLocals noret rid oresult lc = Some lc' ->
   nbInsn 
-    (mkState S TD Ps ((mkEC F B ((insn_call rid noret tailc ft fv lp)::cs) tmn lc
-                       als)::EC) gl fs Mem, tr)
+    (mkState S TD Ps ((mkEC F B ((insn_call rid noret ca ft fv lp)::cs) tmn 
+                       lc als)::EC) gl fs Mem, tr)
     ((mkState S TD Ps ((mkEC F B cs tmn lc' als)::EC) gl fs Mem', tr)::nil)
 
 with nbop_star : States -> States -> Prop :=
@@ -1649,19 +1649,19 @@ with nbop_star : States -> States -> Prop :=
 with nbFdef : value -> typ -> params -> system -> TargetData -> products -> 
   list ExecutionContext -> GVMap -> GVMap -> GVMap -> mem -> trace -> 
   list (GVMap*list mblock*mem*block*id*option value*trace) -> Prop :=
-| nbFdef_intro : forall S TD Ps lc gl fs fv fid lp
+| nbFdef_intro : forall S TD Ps lc gl fs fv fid lp fa
             l' ps' cs' tmn' rt la va lb tr lc_als_Mem_block_rid_ore_trs ECs Mem,
   lookupFdefViaGV TD Mem Ps gl lc fs fv = 
-    Some (fdef_intro (fheader_intro rt fid la va) lb) ->
-  getEntryBlock (fdef_intro (fheader_intro rt fid la va) lb) = 
+    Some (fdef_intro (fheader_intro fa rt fid la va) lb) ->
+  getEntryBlock (fdef_intro (fheader_intro fa rt fid la va) lb) = 
     Some (block_intro l' ps' cs' tmn') ->
   nbop_star 
-    ((mkState S TD Ps ((mkEC (fdef_intro (fheader_intro rt fid la va) lb) 
+    ((mkState S TD Ps ((mkEC (fdef_intro (fheader_intro fa rt fid la va) lb) 
                          (block_intro l' ps' cs' tmn') cs' tmn' 
                          (initLocals la (params2GVs TD Mem lp lc gl)) 
                          nil)::ECs) gl fs Mem, tr)
                          ::nil)
-    (returnStatesFromOp S TD Ps ECs gl fs rt fid la va lb 
+    (returnStatesFromOp S TD Ps ECs gl fs fa rt fid la va lb 
       lc_als_Mem_block_rid_ore_trs) ->
   nbFdef fv rt lp S TD Ps ECs lc gl fs Mem tr lc_als_Mem_block_rid_ore_trs
 .
@@ -1688,13 +1688,13 @@ Inductive nbop_plus : States -> States -> Prop :=
 .
 
 CoInductive nbInsnInf : State*trace -> list Trace -> Prop :=
-| nbCallInsnInf : forall S TD Ps F B lc gl fs rid noret tailc rt fv lp
+| nbCallInsnInf : forall S TD Ps F B lc gl fs rid noret ca rt fv lp
                             EC tr trs Mem als cs tmn ft, 
   nbFdefInf fv rt lp S TD Ps 
-    ((mkEC F B ((insn_call rid noret tailc ft fv lp)::cs) tmn lc als)::EC)  
+    ((mkEC F B ((insn_call rid noret ca ft fv lp)::cs) tmn lc als)::EC)  
     lc gl fs Mem tr trs ->
   nbInsnInf 
-    (mkState S TD Ps ((mkEC F B ((insn_call rid noret tailc ft fv lp)::cs) tmn 
+    (mkState S TD Ps ((mkEC F B ((insn_call rid noret ca ft fv lp)::cs) tmn 
     lc als)::EC) gl fs Mem, tr) trs
 
 with nbopInf : States -> list Trace -> Prop :=
@@ -1710,14 +1710,14 @@ with nbopInf : States -> list Trace -> Prop :=
 with nbFdefInf : value -> typ -> params -> system -> TargetData -> products -> 
                  list ExecutionContext -> GVMap -> GVMap -> GVMap -> mem -> 
                  trace -> list Trace -> Prop :=
-| nbFdefInf_intro : forall S TD Ps lc gl fs fv fid lp
+| nbFdefInf_intro : forall S TD Ps lc gl fs fv fid lp fa
                             l' ps' cs' tmn' ECs rt la va lb tr trs' Mem,
   lookupFdefViaGV TD Mem Ps gl lc fs fv = 
-    Some (fdef_intro (fheader_intro rt fid la va) lb) ->
-  getEntryBlock (fdef_intro (fheader_intro rt fid la va) lb) = 
+    Some (fdef_intro (fheader_intro fa rt fid la va) lb) ->
+  getEntryBlock (fdef_intro (fheader_intro fa rt fid la va) lb) = 
     Some (block_intro l' ps' cs' tmn') ->
   nbopInf 
-    ((mkState S TD Ps ((mkEC (fdef_intro (fheader_intro rt fid la va) lb) 
+    ((mkState S TD Ps ((mkEC (fdef_intro (fheader_intro fa rt fid la va) lb) 
                           (block_intro l' ps' cs' tmn') cs' tmn' 
                           (initLocals la (params2GVs TD Mem lp lc gl)) 
                           nil)::ECs) gl fs Mem, tr)
