src/TV/sub_tv.v
@@ -183,7 +183,7 @@ Definition function_returns_pointer Ps1 fid2 : bool :=
 match (rename_fid_inv fid2) with
 | Some fid1 =>
     match lookupFdefViaIDFromProducts Ps1 fid1 with      
-    | Some (fdef_intro (fheader_intro (typ_pointer _ as tp) _ _ _) _) => true
+    | Some (fdef_intro (fheader_intro _ (typ_pointer _ as tp) _ _ _) _) => true
     | _ => false
     end
 | None => false
@@ -193,7 +193,7 @@ end.
 Definition store_to_ret Ps1 Ps2 fid2 (ptr:sterm) : bool :=
 if (function_returns_pointer Ps1 fid2) then
    match SBsyntax.lookupFdefViaIDFromProducts Ps2 fid2 with      
-   | Some (SBsyntax.fdef_intro (fheader_intro _  _ ((_,re)::_) _) _) =>
+   | Some (SBsyntax.fdef_intro (fheader_intro _ _  _ ((_,re)::_) _) _) =>
        match remove_cast ptr with
        | sterm_gep _ _ (sterm_val (value_id id0)) 
           (Cons_list_sterm (sterm_val (value_const (const_int _ i0)))
@@ -360,14 +360,14 @@ match (tsts1, tsts2) with
 end.
 
 Inductive scall : Set :=
-| stmn_call : id -> noret -> tailc -> typ -> sterm -> list (typ*sterm) -> scall
+| stmn_call : id -> noret -> clattrs -> typ -> sterm -> list (typ*sterm) -> scall
 .
 
 Definition se_call : forall (st : sstate)(i:cmd)(iscall:isCall i = true), scall.
 Proof.
   intros. unfold isCall in iscall.
   destruct i0; try solve [inversion iscall].
-  apply (@stmn_call i0 n t t0 (value2Sterm st.(STerms) v) 
+  apply (@stmn_call i0 n c t (value2Sterm st.(STerms) v) 
                       (list_param__list_typ_subst_sterm p st.(STerms))).
 Defined.
 
@@ -490,13 +490,13 @@ match (bs1, bs2) with
 end.
 
 Definition tv_fheader nts1 (f1 f2:fheader) := 
-  let '(fheader_intro t1 fid1 a1 va1) := f1 in
-  let '(fheader_intro t2 fid2 a2 va2) := f2 in
+  let '(fheader_intro fa1 t1 fid1 a1 va1) := f1 in
+  let '(fheader_intro fa2 t2 fid2 a2 va2) := f2 in
   tv_fid fid1 fid2 &&
   match t1 with
   | typ_pointer _ =>
       match a2 with
-      | (typ_pointer t,_)::a2' =>
+      | (typ_pointer t,_,_)::a2' =>
         match SBsyntax.get_ret_typs nts1 t with
         | Some (t01,t02,t03) =>
             tv_typ t1 t01 && tv_typ t02 t03 && 
@@ -506,9 +506,10 @@ Definition tv_fheader nts1 (f1 f2:fheader) :=
                   gnerates tmp variable names for its arguments started from
                   %0. So we simply check if their types are matched.
                *)
-              let '(ts1,_) := List.split a1 in
-              let '(ts2',_) := List.split a2' in
-              (sumbool2bool _ _ (prefix_dec _ typ_dec ts1 ts2'))
+              let ts1 := args2Typs a1 in
+              let ts2' := args2Typs a2' in
+              (sumbool2bool _ _ (prefix_dec _ typ_dec (unmake_list_typ ts1) 
+                (unmake_list_typ ts2')))
             else 
               (sumbool2bool _ _ (prefix_dec _ arg_dec a1 a2'))
         | None => false
@@ -525,7 +526,7 @@ end.
 
 Definition tv_fdef nts1 Ps1 Ps2 (f1:fdef) (f2:SBsyntax.fdef) :=
 match (f1, f2) with
-| (fdef_intro (fheader_intro _ fid1 _ _ as fh1) lb1, 
+| (fdef_intro (fheader_intro _ _ fid1 _ _ as fh1) lb1, 
    SBsyntax.fdef_intro fh2 lb2) =>
   tv_fheader nts1 fh1 fh2 && tv_blocks Ps1 Ps2 fid1 lb1 lb2
 end.
@@ -1039,7 +1040,7 @@ end.
 
 Definition rtv_fdef nts1 Ps1 Ps2 (f1:fdef) (f2:SBsyntax.fdef) :=
 match (f1, f2) with
-| (fdef_intro (fheader_intro _ fid1 _ _ as fh1) lb1, 
+| (fdef_intro (fheader_intro _ _ fid1 _ _ as fh1) lb1, 
    SBsyntax.fdef_intro fh2 lb2) =>
   match rtv_blocks Ps1 Ps2 fid1 nil lb1 lb2 with
   | None => false
@@ -1556,7 +1557,7 @@ match c2 with
       else
         match (SBsyntax.lookupFdefViaIDFromProducts Ps2 fid2) with
         | None => true
-        | Some (SBsyntax.fdef_intro (fheader_intro _ _ args2 _) _) =>
+        | Some (SBsyntax.fdef_intro (fheader_intro _ _ _ args2 _) _) =>
             mtv_func_metadata (get_metadata tt) Ps2 fid l1 i1 fid2 args2 tsts2
         end
   | _ => true
@@ -1567,7 +1568,7 @@ match c2 with
       if (isCallLib fid2) then true
       else
         match (SBsyntax.lookupFdefViaIDFromProducts Ps2 fid2) with
-        | Some (SBsyntax.fdef_intro (fheader_intro _ _ (_::args2) _) _) =>
+        | Some (SBsyntax.fdef_intro (fheader_intro _ _ _ (_::args2) _) _) =>
             mtv_func_metadata (get_metadata tt) Ps2 fid l1 i1 fid2 args2 tsts2
         | _ => true
         end
@@ -1698,7 +1699,7 @@ end.
 
 Definition mtv_fdef Ps1 Ps2 (f2:SBsyntax.fdef) :=
 match f2 with
-| SBsyntax.fdef_intro ((fheader_intro t2 fid2 a2 _) as fh2) lb2 =>
+| SBsyntax.fdef_intro ((fheader_intro _ t2 fid2 a2 _) as fh2) lb2 =>
   if (isCallLib fid2) then true else mtv_blocks Ps1 Ps2 fid2 lb2
 end.
 
