src/TV/sub_tv_infer.v
@@ -274,11 +274,11 @@ metadata_from_sterms st2.(STerms) accum'.
     call fid2 sars2
   }  
 *)
-Fixpoint lookupSarg (ars2:list (typ*id)) (sars2:list (typ*sterm)) (i:id) :
-  option sterm :=
+Fixpoint lookupSarg (ars2:list (typ*attributes*id)) (sars2:list (typ*sterm)) 
+  (i:id) :option sterm :=
 match (ars2, sars2) with
 | (nil, nil) => None
-| ((_,i')::ars2', (_,s')::sars2') =>
+| ((_,_,i')::ars2', (_,s')::sars2') =>
     if (eq_id i i') then Some s' else lookupSarg ars2' sars2' i
 | _ => None
 end.
@@ -315,20 +315,20 @@ end.
 
 Inductive sicall : Set :=
 | stmn_icall_nptr : 
-    id -> noret -> tailc -> typ -> sterm -> list (typ*sterm) -> sicall
+    id -> noret -> clattrs -> typ -> sterm -> list (typ*sterm) -> sicall
 | stmn_icall_ptr : 
-    id -> noret -> tailc -> typ -> sterm -> list (typ*sterm) ->
+    id -> noret -> clattrs -> typ -> sterm -> list (typ*sterm) ->
     id -> id -> id -> id -> id -> id -> id -> const -> const -> const -> sicall
 .
 
 Definition se_icall (st:sstate) (i:SBsyntax.call) : sicall :=
 match i with
-| SBsyntax.insn_call_nptr id0 nr tc t0 v0 p0 =>
-    stmn_icall_nptr id0 nr tc t0 (value2Sterm st.(STerms) v0) 
+| SBsyntax.insn_call_nptr id0 nr ca t0 v0 p0 =>
+    stmn_icall_nptr id0 nr ca t0 (value2Sterm st.(STerms) v0) 
       (list_param__list_typ_subst_sterm p0 st.(STerms))
-| SBsyntax.insn_call_ptr id0 nr tc t0 v0 p0 sid id1 id2 id3 id4 id5 id6 
+| SBsyntax.insn_call_ptr id0 nr ca t0 v0 p0 sid id1 id2 id3 id4 id5 id6 
     cst0 cst1 cts2 =>
-    stmn_icall_ptr id0 nr tc t0 (value2Sterm st.(STerms) v0) 
+    stmn_icall_ptr id0 nr ca t0 (value2Sterm st.(STerms) v0) 
       (list_param__list_typ_subst_sterm p0 st.(STerms))
       sid id1 id2 id3 id4 id5 id6 cst0 cst1 cts2
 end.
@@ -343,7 +343,7 @@ match c2 with
       else
         match (SBsyntax.lookupFdefViaIDFromProducts Ps2 fid2) with
         | None => accum
-        | Some (SBsyntax.fdef_intro (fheader_intro _ _ args2 _) _) =>
+        | Some (SBsyntax.fdef_intro (fheader_intro _ _ _ args2 _) _) =>
            metadata_from_params (get_arg_metadata flnbep0 fid2) args2 tsts2 accum
         end
   | _ => accum
@@ -354,7 +354,7 @@ match c2 with
       if (isCallLib fid2) then accum
       else
         match (SBsyntax.lookupFdefViaIDFromProducts Ps2 fid2) with
-        | Some (SBsyntax.fdef_intro (fheader_intro _ _ (_::args2) _) _) =>
+        | Some (SBsyntax.fdef_intro (fheader_intro _ _ _ (_::args2) _) _) =>
            metadata_from_params (get_arg_metadata flnbep0 fid2) args2 tsts2 accum
         | _ => accum
         end
@@ -644,7 +644,7 @@ end.
 Definition metadata_from_fdef Ps2 flbep (f2:SBsyntax.fdef) (md:lnbeps) 
   (bsteps:onat) : lnbeps :=
 match f2 with
-| SBsyntax.fdef_intro ((fheader_intro t2 fid2 a2 _) as fh2) lb2 =>
+| SBsyntax.fdef_intro ((fheader_intro _ t2 fid2 a2 _) as fh2) lb2 =>
   if (isCallLib fid2) then md 
   else 
    let accum := metadata_from_blocks Ps2 flbep lb2 
@@ -745,7 +745,7 @@ disjoint_mptr_fptr_metadata_aux (nbeps_to_beps (lnbeps_to_nbeps md nil) nil).
 Definition validate_metadata_from_fdef Ps2 flbep (f2:SBsyntax.fdef) (md:lnbeps) 
   : bool :=
 match f2 with
-| SBsyntax.fdef_intro ((fheader_intro t2 fid2 a2 _) as fh2) lb2 =>
+| SBsyntax.fdef_intro ((fheader_intro _ t2 fid2 a2 _) as fh2) lb2 =>
   if (isCallLib fid2) then true
   else 
     disjoint_mptr_fptr_metadata md &&
@@ -864,7 +864,7 @@ end.
 
 Definition addrofbe_from_fdef (f2:SBsyntax.fdef) (md:abes) : abes :=
 match f2 with
-| SBsyntax.fdef_intro ((fheader_intro t2 fid2 a2 _) as fh2) lb2 =>
+| SBsyntax.fdef_intro ((fheader_intro _ t2 fid2 a2 _) as fh2) lb2 =>
   if (isCallLib fid2) then md 
   else addrofbe_from_blocks lb2 nil
 end.
